some renames

src/Iris/Algebra/View.lean
@@ -14,20 +14,20 @@ import Iris.Algebra.LocalUpdates
 
 open Iris
 
-abbrev view_rel (A B : Type _) := Nat → A → B → Prop
+abbrev ViewRel (A B : Type _) := Nat → A → B → Prop
 
-class ViewRel [OFE A] [UCMRA B] (R : view_rel A B) where
+class IsViewRel [OFE A] [UCMRA B] (R : ViewRel A B) where
   mono : R n1 a1 b1 → a1 ≡{n2}≡ a2 → b2 ≼{n2} b1 → n2 ≤ n1 → R n2 a2 b2
   rel_validN n a b : R n a b → ✓{n} b
   rel_unit n : ∃ a, R n a UCMRA.unit
 
-class ViewRelDiscrete [OFE A] [UCMRA B] (R : view_rel A B) extends ViewRel R where
+class IsViewRelDiscrete [OFE A] [UCMRA B] (R : ViewRel A B) extends IsViewRel R where
   discrete n a b : R 0 a b → R n a b
 
-namespace viewrel
-open ViewRel DFrac
+namespace ViewRel
+open IsViewRel DFrac
 
-variable [OFE A] [UCMRA B] {R : view_rel A B} [ViewRel R]
+variable [OFE A] [UCMRA B] {R : ViewRel A B} [IsViewRel R]
 
 theorem ne (Ha : a1 ≡{n}≡ a2) (Hb : b1 ≡{n}≡ b2) : R n a1 b1 ↔ R n a2 b2 :=
   ⟨(mono · Ha Hb.symm.to_incN n.le_refl), (mono · Ha.symm Hb.to_incN n.le_refl)⟩
@@ -35,16 +35,16 @@ theorem ne (Ha : a1 ≡{n}≡ a2) (Hb : b1 ≡{n}≡ b2) : R n a1 b1 ↔ R n a2 
 theorem eqv_ne (Ha : a1 ≡ a2) (Hb : b1 ≡ b2) : R n a1 b1 ↔ R n a2 b2 :=
   ne Ha.dist Hb.dist
 
-end viewrel
+end ViewRel
 
-structure View (F : Type _) {A B : Type _} (R : view_rel A B) where
-  π_auth : Option ((DFrac F) × Agree A)
-  π_frag : B
+structure View (F : Type _) {A B : Type _} (R : ViewRel A B) where
+  auth : Option ((DFrac F) × Agree A)
+  frag : B
 
-abbrev View.Auth [UCMRA B] {R : view_rel A B} (dq : DFrac F) (a : A) : View F R :=
+abbrev View.Auth [UCMRA B] {R : ViewRel A B} (dq : DFrac F) (a : A) : View F R :=
   ⟨some (dq, toAgree a), UCMRA.unit⟩
 
-abbrev View.Frag {R : view_rel A B} (b : B) : View F R := ⟨none, b⟩
+abbrev View.Frag {R : ViewRel A B} (b : B) : View F R := ⟨none, b⟩
 
 notation "●V{" dq "} " a => View.Auth dq a
 notation "●V " a => View.Auth (DFrac.own One.one) a
@@ -53,10 +53,10 @@ notation "◯V " b => View.Frag b
 namespace View
 section ofe
 
-variable [OFE A] [OFE B] {R : view_rel A B}
+variable [OFE A] [OFE B] {R : ViewRel A B}
 
-abbrev equiv (x y : View F R) : Prop := x.π_auth ≡ y.π_auth ∧ x.π_frag ≡ y.π_frag
-abbrev dist (n : Nat) (x y : View F R) : Prop := x.π_auth ≡{n}≡ y.π_auth ∧ x.π_frag ≡{n}≡ y.π_frag
+abbrev equiv (x y : View F R) : Prop := x.auth ≡ y.auth ∧ x.frag ≡ y.frag
+abbrev dist (n : Nat) (x y : View F R) : Prop := x.auth ≡{n}≡ y.auth ∧ x.frag ≡{n}≡ y.frag
 
 instance : OFE (View F R) where
   Equiv := equiv
@@ -71,45 +71,45 @@ instance : OFE (View F R) where
      fun H => ⟨OFE.equiv_dist.mpr (H · |>.1), OFE.equiv_dist.mpr (H · |>.2)⟩⟩
   dist_lt H Hn := ⟨OFE.dist_lt H.1 Hn, OFE.dist_lt H.2 Hn⟩
 
-instance View.mk.ne : OFE.NonExpansive₂ (View.mk : _ → _ → View F R) := ⟨fun _ _ _ Ha _ _ Hb => ⟨Ha, Hb⟩⟩
-instance View.π_auth.ne : OFE.NonExpansive (View.π_auth : View F R → _) := ⟨fun _ _ _ H => H.1⟩
-instance View.π_frag.ne : OFE.NonExpansive (View.π_frag : View F R → _) := ⟨fun _ _ _ H => H.2⟩
+instance mk.ne : OFE.NonExpansive₂ (mk : _ → _ → View F R) := ⟨fun _ _ _ Ha _ _ Hb => ⟨Ha, Hb⟩⟩
+instance auth.ne : OFE.NonExpansive (auth : View F R → _) := ⟨fun _ _ _ H => H.1⟩
+instance frag.ne : OFE.NonExpansive (frag : View F R → _) := ⟨fun _ _ _ H => H.2⟩
 
-theorem View.is_discrete {ag : Option ((DFrac F) × Agree A)} (Ha : OFE.DiscreteE ag) (Hb : OFE.DiscreteE b) :
-  OFE.DiscreteE (α := View F R) (View.mk ag b) := ⟨fun H => ⟨Ha.discrete H.1, Hb.discrete H.2⟩⟩
+theorem is_discrete {ag : Option ((DFrac F) × Agree A)} (Ha : OFE.DiscreteE ag) (Hb : OFE.DiscreteE b) :
+  OFE.DiscreteE (α := View F R) (mk ag b) := ⟨fun H => ⟨Ha.discrete H.1, Hb.discrete H.2⟩⟩
 
 open OFE in
 instance [Discrete A] [Discrete B] : Discrete (View F R) where
   discrete_0 H := ⟨discrete_0 H.1, discrete_0 H.2⟩
 
-theorem View.auth_inj_frac [UCMRA B] {q1 q2 : DFrac F} {a1 a2 : A} {n} (H : (●V{q1} a1 : View F R) ≡{n}≡ ●V{q2} a2) :
+theorem auth_inj_frac [UCMRA B] {q1 q2 : DFrac F} {a1 a2 : A} {n} (H : (●V{q1} a1 : View F R) ≡{n}≡ ●V{q2} a2) :
     q1 = q2 := H.1.1
 
-theorem View.auth_inj_ag [UCMRA B] {q1 q2 : DFrac F} {a1 a2 : A} {n} (H : (●V{q1} a1 : View F R) ≡{n}≡ ●V{q2} a2) :
+theorem auth_inj_ag [UCMRA B] {q1 q2 : DFrac F} {a1 a2 : A} {n} (H : (●V{q1} a1 : View F R) ≡{n}≡ ●V{q2} a2) :
     a1 ≡{n}≡ a2 := toAgree.inj H.1.2
 
-theorem View.frag_inj [UCMRA B] {b1 b2 : B} {n} (H : (◯V b1 : View F R) ≡{n}≡ ◯V b2) :
+theorem frag_inj [UCMRA B] {b1 b2 : B} {n} (H : (◯V b1 : View F R) ≡{n}≡ ◯V b2) :
     b1 ≡{n}≡ b2 := H.2
 
-theorem View.auth_is_discrete [UFraction F] [UCMRA B] {dq a} (Ha : OFE.DiscreteE a) (He : OFE.DiscreteE (UCMRA.unit : B)) :
+theorem auth_is_discrete [UFraction F] [UCMRA B] {dq a} (Ha : OFE.DiscreteE a) (He : OFE.DiscreteE (UCMRA.unit : B)) :
     OFE.DiscreteE (●V{dq} a : View F R) := by
-  refine View.is_discrete ?_ He
+  refine is_discrete ?_ He
   apply OFE.Option.some_is_discrete
   apply OFE.prod.is_discrete DFrac.is_discrete
   apply Agree.toAgree.is_discrete
   exact Ha
 
-theorem View.frag_is_discrete [UCMRA B] {b : B} (Hb : OFE.DiscreteE b) : (OFE.DiscreteE (◯V b : View F R)) :=
-  View.is_discrete OFE.Option.none_is_discrete Hb
+theorem frag_is_discrete [UCMRA B] {b : B} (Hb : OFE.DiscreteE b) : (OFE.DiscreteE (◯V b : View F R)) :=
+  is_discrete OFE.Option.none_is_discrete Hb
 
 end ofe
 
 section cmra
-open ViewRel toAgree OFE
+open IsViewRel toAgree OFE
 
-variable [UFraction F] [OFE A] [IB : UCMRA B] {R : view_rel A B} [ViewRel R]
+variable [UFraction F] [OFE A] [IB : UCMRA B] {R : ViewRel A B} [IsViewRel R]
 
-theorem ViewRel.of_agree_dst_iff (Hb : b' ≡{n}≡ b) :
+theorem IsViewRel.of_agree_dst_iff (Hb : b' ≡{n}≡ b) :
     (∃ a', toAgree a ≡{n}≡ toAgree a' ∧ R n a' b') ↔ R n a b := by
   refine ⟨fun H => ?_, fun H => ?_⟩
   · rcases H with ⟨_, HA, HR⟩
@@ -118,36 +118,36 @@ theorem ViewRel.of_agree_dst_iff (Hb : b' ≡{n}≡ b) :
 
 instance auth_ne {dq : DFrac F} : NonExpansive (Auth dq : A → View F R) where
   ne _ _ _ H := by
-    refine View.mk.ne.ne ?_ .rfl
+    refine mk.ne.ne ?_ .rfl
     refine some_dist_some.mpr ⟨.rfl, ?_⟩
     simp only
     exact OFE.NonExpansive.ne H
 
 instance auth_ne₂ : NonExpansive₂ (Auth : DFrac F → A → View F R) where
   ne _ _ _ Hq _ _ Hf := by
-    unfold View.Auth
+    unfold Auth
     refine (NonExpansive₂.ne ?_ .rfl)
     refine NonExpansive.ne ?_
     exact dist_prod_ext Hq (NonExpansive.ne Hf)
 
 instance frag_ne : NonExpansive (Frag : B → View F R) where
-  ne _ _ _ H := View.mk.ne.ne .rfl H
+  ne _ _ _ H := mk.ne.ne .rfl H
 
 @[simp] def Valid (v : View F R) : Prop :=
-  match v.π_auth with
-  | some (dq, ag) => ✓ dq ∧ (∀ n, ∃ a, ag ≡{n}≡ toAgree a ∧ R n a (π_frag v))
-  | none => ∀ n, ∃ a, R n a (π_frag v)
+  match v.auth with
+  | some (dq, ag) => ✓ dq ∧ (∀ n, ∃ a, ag ≡{n}≡ toAgree a ∧ R n a (frag v))
+  | none => ∀ n, ∃ a, R n a (frag v)
 
 @[simp] def ValidN (n : Nat) (v : View F R) : Prop :=
-  match v.π_auth with
-  | some (dq, ag) => ✓{n} dq ∧ (∃ a, ag ≡{n}≡ toAgree a ∧ R n a (π_frag v))
-  | none => ∃ a, R n a (π_frag v)
+  match v.auth with
+  | some (dq, ag) => ✓{n} dq ∧ (∃ a, ag ≡{n}≡ toAgree a ∧ R n a (frag v))
+  | none => ∃ a, R n a (frag v)
 
 @[simp] def Pcore (v : View F R) : Option (View F R) :=
-  some <| View.mk (CMRA.core v.1) (CMRA.core v.2)
+  some <| mk (CMRA.core v.auth) (CMRA.core v.frag)
 
 @[simp] def Op (v1 v2 : View F R) : View F R :=
-  View.mk (v1.1 • v2.1) (v1.2 • v2.2)
+  mk (v1.auth • v2.auth) (v1.frag • v2.frag)
 
 instance : CMRA (View F R) where
   pcore := Pcore
@@ -155,25 +155,25 @@ instance : CMRA (View F R) where
   ValidN := ValidN
   Valid := Valid
   op_ne.ne n x1 x2 H := by
-    refine View.mk.ne.ne ?_ ?_
+    refine mk.ne.ne ?_ ?_
     · exact cmraOption.op_ne.ne <| NonExpansive.ne H
     · exact IB.op_ne.ne <| NonExpansive.ne H
   pcore_ne {n x y} cx H := by
     simp only [Pcore, Option.some.injEq]
     rintro ⟨rfl⟩
-    exists ⟨CMRA.core y.π_auth, CMRA.core y.π_frag⟩
+    exists ⟨CMRA.core y.auth, CMRA.core y.frag⟩
     exact ⟨rfl, OFE.Dist.core H.1, OFE.Dist.core H.2⟩
   validN_ne {n x1 x2} := by
     rintro ⟨Hl, Hr⟩
     rcases x1 with ⟨_|⟨q1, ag1⟩, b1⟩ <;>
     rcases x2 with ⟨_|⟨q2, ag2⟩, b2⟩ <;>
     simp_all
-    · exact fun x H => ⟨x, ViewRel.mono H .rfl Hr.symm.to_incN n.le_refl⟩
+    · exact fun x H => ⟨x, IsViewRel.mono H .rfl Hr.symm.to_incN n.le_refl⟩
     intro Hq a Hag HR
     refine ⟨CMRA.discrete_valid <| DFrac_CMRA.validN_ne Hl.1 Hq, ?_⟩
     refine ⟨a, ?_⟩
     refine ⟨Hl.2.symm.trans Hag, ?_⟩
-    refine ViewRel.mono HR .rfl ?_ n.le_refl
+    refine IsViewRel.mono HR .rfl ?_ n.le_refl
     exact Dist.to_incN Hr.symm
   valid_iff_validN {x} := by
     simp only [Valid, ValidN]; split
@@ -185,7 +185,7 @@ instance : CMRA (View F R) where
     · refine fun H => ⟨H.1, ?_⟩
       rcases H.2 with ⟨ag, Ha⟩; exists ag
       refine ⟨Dist.le Ha.1 n.le_succ, ?_⟩
-      exact mono Ha.2 .rfl (CMRA.incN_refl x.π_frag) n.le_succ
+      exact mono Ha.2 .rfl (CMRA.incN_refl x.frag) n.le_succ
     · rintro ⟨z, HR⟩
       exact ⟨z, mono HR .rfl (CMRA.incN_refl _) n.le_succ⟩
   validN_op_left {n x y} := by
@@ -199,12 +199,12 @@ instance : CMRA (View F R) where
       · refine .trans ?_ H
         refine .trans Agree.idemp.symm.dist ?_
         exact CMRA.op_ne.ne <| Agree.op_invN (Agree.validN_ne H.symm trivial)
-      · exact ViewRel.mono Hr .rfl (CMRA.incN_op_left n b1 b2) n.le_refl
+      · exact IsViewRel.mono Hr .rfl (CMRA.incN_op_left n b1 b2) n.le_refl
   assoc := OFE.NonExpansive₂.eqv CMRA.assoc CMRA.assoc
   comm := OFE.NonExpansive₂.eqv CMRA.comm CMRA.comm
   pcore_op_left {x _} := by
     simp only [Pcore, Option.some.injEq]
-    exact fun H => H ▸ OFE.NonExpansive₂.eqv (CMRA.core_op x.π_auth) (CMRA.core_op x.π_frag)
+    exact fun H => H ▸ OFE.NonExpansive₂.eqv (CMRA.core_op x.auth) (CMRA.core_op x.frag)
   pcore_idem {_ cx} := by
     simp only [Pcore, Option.some.injEq, OFE.some_eqv_some]
     rcases cx
@@ -213,19 +213,16 @@ instance : CMRA (View F R) where
     constructor
     · simp only; exact H1 ▸ CMRA.core_idem _
     · exact H2 ▸ CMRA.core_idem _
-
-  -- Here
-
   pcore_op_mono := by
     apply pcore_op_mono_of_core_op_mono
     let f : (Option ((DFrac F) × Agree A) × B) → View F R := fun x => ⟨x.1, x.2⟩
-    let g : View F R → (Option ((DFrac F) × Agree A) × B) := fun x => (x.1, x.2)
+    let g : View F R → (Option ((DFrac F) × Agree A) × B) := fun x => (x.auth, x.frag)
     let opM' (x : View F R) (y : Option (View F R)) : View F R :=
       match y with | some y => Op x y | none => x
 
     have g_pcore_0 {y : View F R} : CMRA.pcore (g y) ≡ g <$> Pcore y := by
       rcases y with ⟨x, b⟩
-      simp only [pcore, Option.map_eq_map, Option.map, g]
+      simp only [Option.map_eq_map, Option.map, g]
       simp [CMRA.pcore, Prod.pcore, optionCore]
       simp [CMRA.pcore_eq_core]
       rfl
@@ -254,23 +251,23 @@ instance : CMRA (View F R) where
     refine ⟨cy', ⟨rfl, ?_⟩⟩
     exists (f x)
   extend {n x y1 y2} Hv He := by
-    let g : View F R → (Option ((DFrac F) × Agree A) × B) := fun x => (x.1, x.2)
+    let g : View F R → (Option ((DFrac F) × Agree A) × B) := fun x => (x.auth, x.frag)
     have H2 := @CMRA.extend _ _ n (g x) (g y1) (g y2) ?G1 He
     case G1 =>
       simp_all [ValidN, CMRA.ValidN, Prod.ValidN, g, optionValidN]
       rcases x with ⟨_|⟨q1, ag1⟩, b1⟩ <;> simp_all only
       · refine ⟨trivial, ?_⟩
         rcases Hv with ⟨_, Ha⟩
-        apply ViewRel.rel_validN _ _ _ Ha
+        apply IsViewRel.rel_validN _ _ _ Ha
       · rcases Hv with ⟨Hq, ⟨a, ⟨Ha1, Ha2⟩⟩⟩
         refine ⟨⟨trivial, ?_⟩, ?_⟩
         · exact Agree.validN_ne Ha1.symm trivial
-        · exact ViewRel.rel_validN _ _ _ Ha2
+        · exact IsViewRel.rel_validN _ _ _ Ha2
     rcases H2 with ⟨z1, z2, Hze, Hz1, Hz2⟩
     exists ⟨z1.1, z1.2⟩
     exists ⟨z2.1, z2.2⟩
 
-instance [OFE.Discrete A] [CMRA.Discrete B] [ViewRelDiscrete R] : CMRA.Discrete (View F R) where
+instance [OFE.Discrete A] [CMRA.Discrete B] [IsViewRelDiscrete R] : CMRA.Discrete (View F R) where
   discrete_valid := by
     simp [CMRA.ValidN, ValidN, CMRA.Valid, Valid]
     intro x
@@ -278,13 +275,13 @@ instance [OFE.Discrete A] [CMRA.Discrete B] [ViewRelDiscrete R] : CMRA.Discrete 
     · rintro ⟨H1, ⟨a, H2, H3⟩⟩
       refine ⟨H1, fun n => ⟨a, ⟨?_, ?_⟩⟩⟩
       · exact OFE.equiv_dist.mp (OFE.Discrete.discrete_0 H2) _
-      · exact ViewRelDiscrete.discrete _ _ _ H3
+      · exact IsViewRelDiscrete.discrete _ _ _ H3
     · rintro ⟨a, H⟩ _
-      exact ⟨a, ViewRelDiscrete.discrete _ _ _ H⟩
+      exact ⟨a, IsViewRelDiscrete.discrete _ _ _ H⟩
 
 instance : UCMRA (View F R) where
   unit := ⟨UCMRA.unit, UCMRA.unit⟩
-  unit_valid := ViewRel.rel_unit
+  unit_valid := IsViewRel.rel_unit
   unit_left_id := ⟨UCMRA.unit_left_id, UCMRA.unit_left_id⟩
   pcore_unit := ⟨by rfl, CMRA.core_eqv_self UCMRA.unit⟩
 
@@ -296,7 +293,7 @@ theorem frag_op_eq : (◯V (b1 • b2) : View F R) = ((◯V b1) • ◯V b2 : Vi
 theorem frag_inc_of_inc (H : b1 ≼ b2) : (◯V b1 : View F R) ≼ ◯V b2 := by
   rcases H with ⟨c, H⟩
   refine CMRA.inc_of_inc_of_eqv ?_ (NonExpansive.eqv H.symm)
-  rw [View.frag_op_eq]
+  rw [frag_op_eq]
   exact CMRA.inc_op_left _ _
 
 theorem core_frag : CMRA.core (◯V b : View F R) = ◯V (CMRA.core b) := rfl
@@ -329,7 +326,7 @@ theorem eqv_of_valid_auth (H : ✓ ((●V{dq1} a1 : View F R) • ●V{dq2} a2))
   OFE.equiv_dist.mpr fun _ => dst_of_validN_auth H.validN
 
 theorem auth_validN_iff : ✓{n} (●V{dq} a : View F R) ↔ ✓{n}dq ∧ R n a UCMRA.unit :=
-  and_congr_right fun _ => ViewRel.of_agree_dst_iff .rfl
+  and_congr_right fun _ => IsViewRel.of_agree_dst_iff .rfl
 
 theorem auth_one_validN_iff n a : ✓{n} (●V a : View F R) ↔ R n a UCMRA.unit :=
   ⟨(auth_validN_iff.mp · |>.2), (auth_validN_iff.mpr ⟨UFraction.one_whole.1, ·⟩)⟩
@@ -339,7 +336,7 @@ theorem auth_op_auth_validN_iff :
   refine ⟨fun H => ?_, fun H => ?_⟩
   · let Ha' : a1 ≡{n}≡ a2 := dst_of_validN_auth H
     rcases H with ⟨Hq, _, Ha, HR⟩
-    refine ⟨Hq, Ha', ViewRel.mono HR ?_ CMRA.incN_unit n.le_refl⟩
+    refine ⟨Hq, Ha', IsViewRel.mono HR ?_ CMRA.incN_unit n.le_refl⟩
     refine .trans ?_ Ha'.symm
     refine toAgree.inj ?_
     apply Ha.symm.trans
@@ -349,7 +346,7 @@ theorem auth_op_auth_validN_iff :
   · simp [CMRA.op, CMRA.ValidN, ValidN, optionOp, Prod.op]
     refine ⟨H.1, a1, ?_, ?_⟩
     · exact (CMRA.op_ne.ne <| toAgree.ne.ne H.2.1.symm).trans Agree.idemp.dist
-    · refine ViewRel.mono H.2.2 .rfl ?_ n.le_refl
+    · refine IsViewRel.mono H.2.2 .rfl ?_ n.le_refl
       exact OFE.Dist.to_incN <| CMRA.unit_left_id_dist UCMRA.unit
 
 theorem auth_one_op_validN_iff : ✓{n} ((●V a1 : View F R) • ●V a2) ↔ False := by
@@ -362,13 +359,13 @@ theorem auth_one_op_validN_iff : ✓{n} ((●V a1 : View F R) • ●V a2) ↔ F
 theorem frag_validN_iff : ✓{n} (◯V b : View F R) ↔ ∃ a, R n a b := by rfl
 
 theorem auth_op_frag_validN_iff : ✓{n} ((●V{dq} a : View F R) • ◯V b) ↔ ✓dq ∧ R n a b :=
-  and_congr_right (fun _ => ViewRel.of_agree_dst_iff <| CMRA.unit_left_id_dist b)
+  and_congr_right (fun _ => IsViewRel.of_agree_dst_iff <| CMRA.unit_left_id_dist b)
 
 theorem auth_one_op_frag_validN_iff : ✓{n} ((●V a : View F R) • ◯V b) ↔ R n a b :=
   auth_op_frag_validN_iff.trans <| and_iff_right_iff_imp.mpr (fun _ => valid_own_one)
 
 theorem auth_valid_iff : ✓ (●V{dq} a : View F R) ↔ ✓dq ∧ ∀ n, R n a UCMRA.unit :=
-  and_congr_right (fun _=> forall_congr' fun _ => ViewRel.of_agree_dst_iff .rfl)
+  and_congr_right (fun _=> forall_congr' fun _ => IsViewRel.of_agree_dst_iff .rfl)
 
 theorem auth_one_valid_iff : ✓ (●V a : View F R) ↔ ∀ n, R n a UCMRA.unit :=
   auth_valid_iff.trans <| and_iff_right_iff_imp.mpr (fun _ => valid_own_one)
@@ -376,11 +373,11 @@ theorem auth_one_valid_iff : ✓ (●V a : View F R) ↔ ∀ n, R n a UCMRA.unit
 theorem auth_op_auth_valid_iff : ✓ ((●V{dq1} a1 : View F R) • ●V{dq2} a2) ↔ ✓(dq1 • dq2) ∧ a1 ≡ a2 ∧ ∀ n, R n a1 UCMRA.unit := by
   refine CMRA.valid_iff_validN.trans ?_
   refine ⟨fun H => ?_, fun H n => ?_⟩
-  · simp [CMRA.Valid, valid, Auth, CMRA.op, op, optionOp, CMRA.ValidN, ValidN] at H
+  · simp [valid, CMRA.op, op, optionOp, CMRA.ValidN, ValidN] at H
     let Hn (n) := dst_of_validN_auth (H n)
     refine ⟨(H 0).1, OFE.equiv_dist.mpr Hn, fun n => ?_⟩
     · rcases (H n) with ⟨_, _, Hl, H⟩
-      apply ViewRel.mono H ?_ CMRA.incN_unit n.le_refl
+      apply IsViewRel.mono H ?_ CMRA.incN_unit n.le_refl
       apply toAgree.inj
       apply Hl.symm.trans
       exact (CMRA.op_ne.ne <| toAgree.ne.ne (Hn _).symm).trans Agree.idemp.dist
@@ -396,14 +393,14 @@ theorem auth_one_op_auth_one_valid_iff : ✓ ((●V a1 : View F R) • ●V a2) 
 theorem frag_valid_iff : ✓ (◯V b : View F R) ↔ ∀ n, ∃ a, R n a b := by rfl
 
 theorem auth_op_frag_valid_iff : ✓ ((●V{dq} a : View F R) • ◯V b) ↔ ✓dq ∧ ∀ n, R n a b :=
-  and_congr_right (fun _ => forall_congr' fun _ => ViewRel.of_agree_dst_iff <| CMRA.unit_left_id_dist b)
+  and_congr_right (fun _ => forall_congr' fun _ => IsViewRel.of_agree_dst_iff <| CMRA.unit_left_id_dist b)
 
 theorem auth_one_op_frag_valid_iff : ✓ ((●V a : View F R) • ◯V b) ↔ ∀ n, R n a b :=
   auth_op_frag_valid_iff.trans <| and_iff_right_iff_imp.mpr (fun _ => valid_own_one)
 
 theorem auth_incN_auth_op_frag_iff : (●V{dq1} a1 : View F R) ≼{n} ((●V{dq2} a2) • ◯V b) ↔ (dq1 ≼ dq2 ∨ dq1 = dq2) ∧ a1 ≡{n}≡ a2 := by
   refine ⟨?_, ?_⟩
-  · simp only [Auth, Frag, CMRA.IncludedN, CMRA.op, op, optionOp, Prod.op]
+  · simp only [Auth, Frag, CMRA.IncludedN, CMRA.op]
     rintro ⟨(_|⟨dqf, af⟩),⟨⟨x1, x2⟩, y⟩⟩
     · exact ⟨Or.inr x1.symm, toAgree.inj x2.symm⟩
     · simp_all only []
@@ -426,7 +423,7 @@ theorem auth_incN_auth_op_frag_iff : (●V{dq1} a1 : View F R) ≼{n} ((●V{dq2
       case G =>
         apply CMRA.op_ne.ne
         apply OFE.equiv_dist.mp
-        apply View.auth_op_eqv.symm
+        apply auth_op_eqv.symm
       apply (CMRA.incN_iff_right <| ?G).mp
       case G =>
         apply CMRA.op_ne.ne
@@ -481,21 +478,21 @@ theorem auth_one_inc_auth_one_op_frag_iff : (●V a1 : View F R) ≼ ((●V a2) 
 theorem frag_incN_auth_frag_iff : (◯V b1 : View F R) ≼{n} ((●V{p} a) • ◯V b2) ↔ b1 ≼{n} b2 := by
   constructor
   · rintro ⟨xf, ⟨_, Hb⟩⟩
-    simp [Auth, Frag, CMRA.op, op] at Hb
-    have Hb' : b2 ≡{n}≡ b1 • xf.π_frag := by
+    simp [CMRA.op] at Hb
+    have Hb' : b2 ≡{n}≡ b1 • xf.frag := by
       apply OFE.Dist.trans
       apply OFE.Dist.symm
       apply OFE.equiv_dist.mp
       apply UCMRA.unit_left_id
       apply Hb
     apply (CMRA.incN_iff_right <| Hb'.symm).mp
-    exists xf.π_frag
+    exists xf.frag
   · rintro ⟨bf, Hbf⟩
     apply (CMRA.incN_iff_right <| ?G).mp
     case G =>
       apply CMRA.op_ne.ne
       apply NonExpansive.ne Hbf.symm
-    rw [View.frag_op_eq]
+    rw [frag_op_eq]
     apply (CMRA.incN_iff_right <| ?G).mp
     case G =>
       apply OFE.equiv_dist.mp
@@ -509,20 +506,20 @@ theorem frag_incN_auth_frag_iff : (◯V b1 : View F R) ≼{n} ((●V{p} a) • �
 theorem frag_inc_auth_op_frag : (◯V b1 : View F R) ≼ ((●V{p} a) • ◯V b2) ↔ b1 ≼ b2 := by
   constructor
   · rintro ⟨xf, ⟨_, Hb⟩⟩
-    simp [Auth, Frag, CMRA.op, op] at Hb
-    have Hb' : b2 ≡ b1 • xf.π_frag := by
+    simp [CMRA.op] at Hb
+    have Hb' : b2 ≡ b1 • xf.frag := by
       apply OFE.Equiv.trans
       apply OFE.Equiv.symm
       apply UCMRA.unit_left_id
       apply Hb
     apply (CMRA.inc_iff_right <| Hb'.symm).mp
-    exists xf.π_frag
+    exists xf.frag
   · rintro ⟨bf, Hbf⟩
     apply (CMRA.inc_iff_right <| ?G).mp
     case G =>
       apply CMRA.op_ne.eqv
       apply NonExpansive.eqv Hbf.symm
-    rw [View.frag_op_eq]
+    rw [frag_op_eq]
     apply (CMRA.inc_iff_right <| ?G).mp
     case G => apply CMRA.comm
     apply (CMRA.inc_iff_right <| ?G).mp
@@ -552,7 +549,7 @@ theorem auth_op_frag_incN_auth_op_frag_iff :
       apply H2.trans
       apply OFE.equiv_dist.mp
       apply CMRA.comm
-    rewrite [View.frag_op_eq]
+    rewrite [frag_op_eq]
     apply (CMRA.incN_iff_right <| ?G).mp
     case G =>
       apply OFE.equiv_dist.mp
@@ -581,7 +578,7 @@ theorem auth_op_frag_inc_auth_op_frag_iff : ((●V{dq1} a1 : View F R) • ◯V 
       apply OFE.Equiv.symm
       apply H2.trans
       apply CMRA.comm
-    rewrite [View.frag_op_eq]
+    rewrite [frag_op_eq]
     apply (CMRA.inc_iff_right <| ?G).mp
     case G =>
       apply CMRA.assoc.symm
@@ -599,7 +596,7 @@ end cmra
 
 section updates
 
-variable [UFraction F] [OFE A] [IB : UCMRA B] {R : view_rel A B} [ViewRel R]
+variable [UFraction F] [OFE A] [IB : UCMRA B] {R : ViewRel A B} [IsViewRel R]
 
 theorem auth_op_frag_update {Pab : A → B → Prop}
     (Hup : ∀ n bf, R n a (b • bf) → ∃ a' b', Pab a' b' ∧ R n a' (b' • bf)) :
@@ -607,11 +604,11 @@ theorem auth_op_frag_update {Pab : A → B → Prop}
   refine UpdateP.total.mpr (fun n ⟨ag, bf⟩ => ?_)
   rcases ag with (_|⟨dq, ag⟩)
   · intro H
-    simp [CMRA.op, op, CMRA.ValidN, optionOp, ValidN] at H
+    simp [CMRA.op, CMRA.ValidN, optionOp, ValidN] at H
     obtain ⟨_, a0, He', Hrel'⟩ := H
     have He := toAgree.inj He'; clear He'
     have Hrel : R n a (b • bf) := by
-      apply ViewRel.mono Hrel' He.symm _ n.le_refl
+      apply IsViewRel.mono Hrel' He.symm _ n.le_refl
       apply Iris.OFE.Dist.to_incN
       refine CMRA.comm.dist.trans (.trans ?_ CMRA.comm.dist)
       refine CMRA.op_ne.ne ?_
@@ -620,8 +617,8 @@ theorem auth_op_frag_update {Pab : A → B → Prop}
     refine ⟨((●V a') • ◯V b'), ?_, ⟨by trivial, ?_⟩⟩
     · exists a'; exists b'
     · refine ⟨a', .rfl, ?_⟩
-      apply ViewRel.mono Hrel'' .rfl _ n.le_refl
-      simp [CMRA.op, op]
+      apply IsViewRel.mono Hrel'' .rfl _ n.le_refl
+      simp [CMRA.op]
       apply Iris.OFE.Dist.to_incN
       refine CMRA.comm.dist.trans (.trans ?_ CMRA.comm.dist)
       refine CMRA.op_ne.ne ?_
@@ -643,14 +640,14 @@ theorem auth_one_op_frag_update (Hup : ∀ n bf, R n a (b • bf) → R n a' (b'
 theorem auth_one_alloc (Hup : ∀ n bf, R n a bf → R n a' (b' • bf)) :
     ((●V a) ~~> ((●V a' : View F R) • ◯V b')) := by
   refine Update.equiv_left CMRA.unit_right_id ?_
-  refine auth_one_op_frag_update (fun n bf H => Hup n bf <| ViewRel.mono H .rfl ?_ n.le_refl)
+  refine auth_one_op_frag_update (fun n bf H => Hup n bf <| IsViewRel.mono H .rfl ?_ n.le_refl)
   exact CMRA.incN_op_right n UCMRA.unit bf
 
 theorem auth_one_op_frag_dealloc (Hup : (∀ n bf, R n a (b • bf) → R n a' bf)) :
     ((●V a : View F R) • ◯V b) ~~> ●V a' := by
   refine Update.equiv_right CMRA.unit_right_id ?_
   refine auth_one_op_frag_update (fun n bf H => ?_)
-  refine ViewRel.mono (Hup n bf H) .rfl ?_ n.le_refl
+  refine IsViewRel.mono (Hup n bf H) .rfl ?_ n.le_refl
   exact Iris.OFE.Dist.to_incN (CMRA.unit_left_id_dist bf)
 
 theorem auth_one_update (Hup : ∀ n bf, R n a bf → R n a' bf) :
@@ -658,7 +655,7 @@ theorem auth_one_update (Hup : ∀ n bf, R n a bf → R n a' bf) :
   refine Update.equiv_right CMRA.unit_right_id ?_
   refine Update.equiv_left  CMRA.unit_right_id ?_
   refine auth_one_op_frag_update (fun n bf H => ?_)
-  exact ViewRel.mono (Hup n _ H) .rfl .rfl n.le_refl
+  exact IsViewRel.mono (Hup n _ H) .rfl .rfl n.le_refl
 
 theorem auth_update (Hupd : dq ~~>: P) :
     (●V{dq} a : View F R ) ~~>: (fun k => ∃ dq', (k = ●V{dq'} a) ∧ P dq') := by
@@ -705,7 +702,7 @@ theorem frag_updateP {P : B → Prop} (Hupd : ∀ a n bf, R n a (b • bf) → �
     exists (◯V b')
     simp only [mk.injEq, true_and, exists_eq_left']
     refine ⟨Hb', ?_⟩
-    simp [CMRA.ValidN, ValidN, CMRA.op, op, optionOp]
+    simp [CMRA.ValidN, ValidN, CMRA.op, optionOp]
     refine ⟨Hq, ⟨a, Hae, Hp⟩⟩
 
 theorem frag_update (Hupd : ∀ a n bf, R n a (b • bf) → R n a (b' • bf)) :
@@ -717,7 +714,7 @@ theorem frag_update (Hupd : ∀ a n bf, R n a (b • bf) → R n a (b' • bf)) 
     intro a HR
     exists a
     apply Hupd _ _ _ HR
-  · simp_all [CMRA.op, op, optionOp, CMRA.ValidN, ValidN]
+  · simp_all [CMRA.op, optionOp, CMRA.ValidN, ValidN]
     intro Hq a He Hr
     exists a
     exact ⟨He, Hupd _ _ _ Hr⟩
@@ -726,12 +723,12 @@ theorem auth_alloc (Hup : ∀ n bf, R n a bf → R n a (b • bf)) :
     (●V{dq} a : View F R) ~~> ((●V{dq} a) • ◯V b) := by
   refine Update.total.mpr (fun n ⟨ag', bf⟩ => ?_)
   obtain (_|⟨p, ag⟩) := ag'
-  · simp [CMRA.op, op, optionOp, CMRA.ValidN, ValidN]
+  · simp [CMRA.op, optionOp, CMRA.ValidN, ValidN]
     intro Hq a' Hag HR
     refine ⟨Hq, a', Hag, ?_⟩
     have He := toAgree.inj Hag
-    have HR' := ViewRel.mono HR He.symm (CMRA.incN_op_right n UCMRA.unit bf) n.le_refl
-    apply ViewRel.mono (Hup n bf HR') He ?_ n.le_refl
+    have HR' := IsViewRel.mono HR He.symm (CMRA.incN_op_right n UCMRA.unit bf) n.le_refl
+    apply IsViewRel.mono (Hup n bf HR') He ?_ n.le_refl
     apply Iris.OFE.Dist.to_incN
     refine CMRA.comm.dist.trans (.trans ?_ CMRA.comm.dist)
     refine CMRA.op_ne.ne ?_
@@ -743,8 +740,8 @@ theorem auth_alloc (Hup : ∀ n bf, R n a bf → R n a (b • bf)) :
     refine ⟨Hag, ?_⟩
     simp_all [CMRA.op, op]
     have Heq  := toAgree.incN.mp ⟨ag, Hag.symm⟩
-    have HR' := ViewRel.mono Hrel Heq.symm (CMRA.incN_op_right n UCMRA.unit bf) n.le_refl
-    apply ViewRel.mono (Hup _ _ HR') Heq ?_ n.le_refl
+    have HR' := IsViewRel.mono Hrel Heq.symm (CMRA.incN_op_right n UCMRA.unit bf) n.le_refl
+    apply IsViewRel.mono (Hup _ _ HR') Heq ?_ n.le_refl
     apply Iris.OFE.Dist.to_incN
     refine CMRA.comm.dist.trans (.trans ?_ CMRA.comm.dist)
     refine CMRA.op_ne.ne ?_
